1

softwarefoundations/vol2_plf/StlcProp.v
@@ -3,5 +3,654 @@ From PLF Require Import Maps.
 From PLF Require Import Types.
 From PLF Require Import Stlc.
 From PLF Require Import Smallstep.
+
 Module STLCProp.
 Import STLC.
+
+Lemma canonical_forms_bool : forall t,
+  empty |- t \in Bool ->
+  value t ->
+  (t = <{true}>) \/ (t = <{false}>).
+Proof. intros t Ht Hv.
+  inversion Hv.
+  - subst. inversion Ht.
+  - left. reflexivity.
+  - right. reflexivity.
+Qed.
+
+Lemma canonical_forms_fun : forall t T1 T2,
+  empty |- t \in (T1 -> T2) ->
+  value t ->
+  exists x u, t = <{\x:T1, u}>.
+Proof. intros t T1 T2 Ht Hv.
+  inversion Hv; subst.
+  - exists x0, t1. inversion Ht; subst. reflexivity.
+  - inversion Ht. 
+  - inversion Ht. 
+Qed.
+
+Theorem progress : forall t T,
+  empty |- t \in T ->
+  value t \/ exists t', t --> t'.
+Proof. intros t T Ht.
+  remember empty as e eqn:Ee.
+  induction Ht; subst.
+  - (*var*) discriminate H.
+  - (*abs*) left. constructor.
+  - (*app*)
+    destruct IHHt1; try reflexivity.
+    + (*t1 value*)
+      destruct IHHt2; try reflexivity.
+      * (*t2 value*)
+        right. 
+        inversion H; subst; try (inversion Ht1; subst). 
+        exists <{ [x0:=t2]t0 }>. 
+        apply ST_AppAbs. 
+        assumption.
+      * (*t2 progress*)
+        right.
+        destruct H0 as [t' Hr].
+        exists <{t1 t'}>.
+        apply ST_App2.
+        apply H.
+        apply Hr.
+    + (*t1 progress*)
+      right.
+      destruct H as [t' Hr].
+      exists <{t' t2}>.
+      apply ST_App1.
+      apply Hr.
+  - (*true*) left. constructor.
+  - (*false*) left. constructor.
+  - (*if*)
+    right.
+    destruct IHHt1; try reflexivity.
+    + (*t1 val*) 
+      inversion H; subst; try (inversion Ht1; subst).
+      * eexists. apply ST_IfTrue. 
+      * eexists. apply ST_IfFalse. 
+    + (*t1 progr*) destruct H as [t' H]. eexists.
+      apply ST_If. apply H.
+Qed.
+
+Theorem progress' : forall t T,
+     empty |- t \in T ->
+     value t \/ exists t', t --> t'.
+Proof.
+  intros t.
+  induction t; intros T Ht; auto.
+  - (*var*) inversion Ht. discriminate H1.
+  - (*app*) inversion Ht; subst. 
+    destruct (IHt1 _ H2).
+    + (*t1 val*) destruct (IHt2 _ H4).
+      * (*t2 val*) inversion H; subst; try (inversion H2; subst).
+        right.
+        exists <{ [x0:=t2]t0 }>.
+        constructor. assumption.
+      * (*t2 progr*) right.
+        destruct H0 as [t' Ht'].
+        exists <{ t1 t' }>.
+        apply ST_App2. assumption.
+        apply Ht'.
+    + (*t1 progr*)
+      destruct H as [t' Ht'].
+      right. exists <{ t' t2 }>.
+      apply ST_App1. assumption.
+  - (*if*)
+    right.
+    inversion Ht; subst.
+    destruct (IHt1 <{Bool}>); try assumption.
+    + (*t1 val*) 
+      inversion H; subst; try (inversion H3; subst).
+      * eexists. apply ST_IfTrue. 
+      * eexists. apply ST_IfFalse. 
+    + (*t1 progr*) destruct H as [t' H]. eexists.
+      apply ST_If. apply H.
+Qed.
+
+
+
+Lemma weakening : forall Gamma Gamma' t T,
+     inclusion Gamma Gamma' ->
+     Gamma |- t \in T ->
+     Gamma' |- t \in T.
+Proof.
+  intros Gamma Gamma' t T H Ht.
+  generalize dependent Gamma'.
+  induction Ht; eauto using inclusion_update.
+Qed.
+
+Lemma weakening_empty : forall Gamma t T,
+     empty |- t \in T ->
+     Gamma |- t \in T.
+Proof.
+  intros Gamma t T.
+  eapply weakening.
+  discriminate.
+Qed.
+
+Lemma substitution_preserves_typing : forall Gamma x U t v T,
+  (x |-> U ; Gamma) |-  t \in T ->
+  empty |- v \in U ->
+  Gamma |- [x:=v]t \in T.
+Proof.
+  intros Gamma x U t v T Ht Hv.
+  generalize dependent Gamma. generalize dependent T.
+  induction t; intros T Gamma H;
+  (* in each case, we'll want to get at the derivation of H *)
+    inversion H; clear H; subst; simpl; eauto.
+  - (* var *)
+    rename s into y. destruct (eqb_stringP x y); subst.
+    + (* x=y *)
+      rewrite update_eq in H2.
+      injection H2 as H2; subst.
+      apply weakening_empty. assumption.
+    + (* x<>y *)
+      apply T_Var. rewrite update_neq in H2; auto.
+  - (* abs *)
+    rename s into y, t into S.
+    destruct (eqb_stringP x y); subst; apply T_Abs.
+    + (* x=y *)
+      rewrite update_shadow in H5. assumption.
+    + (* x<>y *)
+      apply IHt.
+      rewrite update_permute; auto.
+Qed.
+
+Lemma substitution_preserves_typing_from_typing_ind : forall Gamma x U t v T,
+  (x |-> U ; Gamma) |- t \in T  ->
+  empty |- v \in U  ->
+  Gamma |- [x:=v]t \in T.
+Proof.
+  intros Gamma x U t v T Ht Hv.
+  remember (x |-> U; Gamma) as Gamma'.
+  generalize dependent Gamma.
+  induction Ht; intros Gamma' G; simpl; eauto.
+  - rename x0 into y. destruct (eqb_stringP x y); subst.
+    + rewrite update_eq in H. injection H as H'. subst. apply weakening_empty. assumption.
+    + rewrite update_neq in H. constructor. assumption.
+      assumption.
+  - rename x0 into y. destruct (eqb_stringP x y); subst.
+    + apply T_Abs.
+      rewrite update_shadow in Ht. assumption.
+    + apply T_Abs.
+      apply IHHt.
+      rewrite update_permute; auto.
+Qed.
+
+
+Theorem preservation : forall t t' T,
+  empty |- t \in T ->
+  t --> t' ->
+  empty |- t' \in T.
+Proof with eauto.
+  intros t t' T HT. generalize dependent t'.
+  remember empty as Gamma.
+  induction HT;
+       intros t' HE; subst;
+       try solve [inversion HE; subst; auto].
+  - (* T_App *)
+    inversion HE; subst...
+    (* Most of the cases are immediate by induction,
+       and eauto takes care of them *)
+    + (* ST_AppAbs *)
+      apply substitution_preserves_typing with T2...
+      inversion HT1...
+Qed.
+
+Definition stuck (t:tm) : Prop :=  (normal_form step) t /\ ~(value t).
+Corollary type_soundness : forall t t' T,
+  empty |- t \in T ->
+  t -->* t' ->
+  ~(stuck t').
+Proof.
+  intros t t' T Hhas_type Hmulti. unfold stuck.
+  intros [Hnf Hnot_val]. unfold normal_form in Hnf.
+  induction Hmulti.
+  - apply progress in Hhas_type.
+    destruct Hhas_type as [Hval | Hprogr].
+    + apply Hnot_val. assumption.
+    + apply Hnf. assumption.
+  - apply IHHmulti; try assumption.
+    apply preservation with x0; try assumption.
+Qed.
+
+
+Theorem unique_types : forall Gamma e T T',
+  Gamma |- e \in T  ->
+  Gamma |- e \in T' ->
+  T = T'.
+Proof.
+  intros G e.
+  generalize dependent G.
+  induction e; intros G T T' H H'.
+  - (*var*) inversion H; subst. inversion H'; subst.
+    rewrite H2 in H3. injection H3 as H3. assumption.
+  - (*app*) inversion H; subst. inversion H'; subst.
+    assert (Hg: (<{T2 -> T}>) = (<{T0 -> T'}>)). {
+      apply (IHe1 G). assumption. assumption.
+    }
+    injection Hg as Hg1 Hg2.
+    assumption.
+  - (*abs*) inversion H; subst. inversion H'; subst.
+    assert (Hg: T1 = T0). {
+      eapply IHe.
+      apply H5.
+      apply H6.
+    }
+    rewrite Hg.
+    reflexivity.
+  - (*true*) inversion H; subst. inversion H'; subst.
+    reflexivity.
+  - (*false*) inversion H; subst. inversion H'; subst.
+    reflexivity.
+  - (*if*) inversion H; subst. inversion H'; subst.
+    apply (IHe2 G).
+    assumption.
+    assumption.
+Qed.
+
+
+
+
+Inductive appears_free_in (x : string) : tm -> Prop :=
+  | afi_var : appears_free_in x <{x}>
+  | afi_app1 : forall t1 t2,
+      appears_free_in x t1 ->
+      appears_free_in x <{t1 t2}>
+  | afi_app2 : forall t1 t2,
+      appears_free_in x t2 ->
+      appears_free_in x <{t1 t2}>
+  | afi_abs : forall y T1 t1,
+      y <> x ->
+      appears_free_in x t1 ->
+      appears_free_in x <{\y:T1, t1}>
+  | afi_if1 : forall t1 t2 t3,
+      appears_free_in x t1 ->
+      appears_free_in x <{if t1 then t2 else t3}>
+  | afi_if2 : forall t1 t2 t3,
+      appears_free_in x t2 ->
+      appears_free_in x <{if t1 then t2 else t3}>
+  | afi_if3 : forall t1 t2 t3,
+      appears_free_in x t3 ->
+      appears_free_in x <{if t1 then t2 else t3}>.
+Hint Constructors appears_free_in : core.
+
+Definition closed (t:tm) :=   forall x, ~(appears_free_in x t).
+
+Lemma free_in_context : forall x t T Gamma,
+   appears_free_in x t ->
+   Gamma |- t \in T ->
+   exists T', Gamma x = Some T'.
+Proof.
+  intros x t T G H.
+  generalize dependent G.
+  generalize dependent T.
+  induction H; intros T G Ht; inversion Ht; subst.
+  - exists T.  assumption.
+  - apply IHappears_free_in in H3. assumption.
+  - apply IHappears_free_in in H5. assumption.
+  - apply IHappears_free_in in H6. rewrite update_neq in H6.
+    assumption.
+    assumption.
+  - apply IHappears_free_in in H4. assumption.
+  - apply IHappears_free_in in H6. assumption.
+  - apply IHappears_free_in in H7. assumption.
+Qed.
+
+Corollary typable_empty__closed : forall t T,
+    empty |- t \in T ->
+    closed t.
+Proof.
+  intros t T Ht x Hfr.
+  inversion Ht; subst.
+  - discriminate H.
+  - inversion Hfr; subst.
+    destruct (free_in_context _ _ _ _ H4 H) as [T' Hgt'].
+    rewrite update_neq in Hgt'.
+    + discriminate Hgt'.
+    + assumption.
+  - inversion Hfr; subst.
+    + destruct (free_in_context _ _ _ _ H2 H) as [T' Hgt'].
+      discriminate Hgt'.
+    + destruct (free_in_context _ _ _ _ H2 H0) as [T' Hgt'].
+      discriminate Hgt'.
+  - inversion Hfr.
+  - inversion Hfr.
+  - inversion Hfr; subst.
+    + destruct (free_in_context _ _ _ _ H3 H) as [T' Hgt'].
+      discriminate Hgt'.
+    + destruct (free_in_context _ _ _ _ H3 H0) as [T' Hgt'].
+      discriminate Hgt'.
+    + destruct (free_in_context _ _ _ _ H3 H1) as [T' Hgt'].
+      discriminate Hgt'.
+Qed.
+
+Lemma context_invariance : forall Gamma Gamma' t T,
+     Gamma |- t \in T ->
+     (forall x, appears_free_in x t -> Gamma x = Gamma' x) ->
+     Gamma' |- t \in T.
+Proof.
+  intros G G' t T Ht.
+  generalize dependent G'.
+  induction Ht; intros G' F.
+  - constructor.
+    rewrite <- (F x0).
+      assumption.
+      constructor.
+  - apply T_Abs.
+    apply IHHt.
+    intros x' Hx'.
+    destruct (eqb_stringP x0 x').
+    + subst. rewrite update_eq. rewrite update_eq. reflexivity.
+    + rewrite update_neq; try apply n.
+      rewrite update_neq; try apply n.
+      apply (F x').
+      constructor.
+        apply n.
+        assumption.
+  - apply T_App with T2.
+    + apply IHHt1. intros x' H'. apply F. apply afi_app1. assumption.
+    + apply IHHt2. intros x' H'. apply F. apply afi_app2. assumption.
+  - constructor.
+  - constructor.
+  - constructor.
+    + apply IHHt1. intros x' H'. apply F. apply afi_if1. assumption.
+    + apply IHHt2. intros x' H'. apply F. apply afi_if2. assumption.
+    + apply IHHt3. intros x' H'. apply F. apply afi_if3. assumption.
+Qed.
+
+(*TODO ex *)
+
+End STLCProp.
+
+
+
+Module STLCArith.
+Import STLC.
+
+Inductive ty : Type :=
+  | Ty_Arrow : ty -> ty -> ty
+  | Ty_Nat : ty.
+
+Inductive tm : Type :=
+  | tm_var : string -> tm
+  | tm_app : tm -> tm -> tm
+  | tm_abs : string -> ty -> tm -> tm
+  | tm_const : nat -> tm
+  | tm_succ : tm -> tm
+  | tm_pred : tm -> tm
+  | tm_mult : tm -> tm -> tm
+  | tm_if0 : tm -> tm -> tm -> tm.
+
+Notation "{ x }" := x (in custom stlc at level 1, x constr).
+Notation "<{ e }>" := e (e custom stlc at level 99).
+Notation "( x )" := x (in custom stlc, x at level 99).
+Notation "x" := x (in custom stlc at level 0, x constr at level 0).
+Notation "S -> T" := (Ty_Arrow S T) (in custom stlc at level 50, right associativity).
+Notation "x y" := (tm_app x y) (in custom stlc at level 1, left associativity).
+Notation "\ x : t , y" :=
+  (tm_abs x t y) (in custom stlc at level 90, x at level 99, t custom stlc at level 99, y custom stlc at level 99, left associativity).
+Coercion tm_var : string >-> tm.
+Notation "'Nat'" := Ty_Nat (in custom stlc at level 0).
+Notation "'succ' x" := (tm_succ x) (in custom stlc at level 0,
+                                     x custom stlc at level 0).
+Notation "'pred' x" := (tm_pred x) (in custom stlc at level 0,
+                                     x custom stlc at level 0).
+Notation "x * y" := (tm_mult x y) (in custom stlc at level 1,
+                                      left associativity).
+Notation "'if0' x 'then' y 'else' z" :=
+  (tm_if0 x y z) (in custom stlc at level 89, x custom stlc at level 99, y custom stlc at level 99, z custom stlc at level 99, left associativity).
+Coercion tm_const : nat >-> tm.
+
+Inductive value : tm -> Prop :=
+  | v_abs : forall x T2 t1,
+      value <{ \x:T2, t1 }>
+  | v_nat : forall (x: nat),
+      value <{ x }>.
+Hint Constructors value : core.
+
+Reserved Notation "'[' x ':=' s ']' t" (in custom stlc at level 20, x constr).
+Fixpoint subst (x : string) (s : tm) (t : tm) : tm :=
+  match t with
+  | tm_var y =>
+      if eqb_string x y then s else t
+  | <{t1 t2}> => <{([x:=s] t1) ([x:=s] t2)}>
+  | <{\y:T, t1}> =>
+      if eqb_string x y then t else <{\y:T, [x:=s] t1}>
+  | tm_const n => tm_const n
+  | <{succ t}> => <{succ ([x:=s]t)}>
+  | <{pred t}> => <{pred ([x:=s]t)}>
+  | <{t1 * t2}> => <{([x:=s]t1) * ([x:=s]t2)}>
+  | <{if0 t1 then t2 else t3}> =>
+      <{if0 ([x:=s] t1) then ([x:=s] t2) else ([x:=s] t3)}>
+  end
+where "'[' x ':=' s ']' t" := (subst x s t) (in custom stlc).
+
+Reserved Notation "t '-->' t'" (at level 40).
+Inductive step : tm -> tm -> Prop :=
+  | ST_AppAbs : forall x T2 t1 v2,
+         value v2 ->
+         <{(\x:T2, t1) v2}> --> <{ [x:=v2]t1 }>
+  | ST_App1 : forall t1 t1' t2,
+         t1 --> t1' ->
+         <{t1 t2}> --> <{t1' t2}>
+  | ST_App2 : forall v1 t2 t2',
+         value v1 ->
+         t2 --> t2' ->
+         <{v1 t2}> --> <{v1 t2'}>
+
+  | ST_Pred_0 :
+         <{pred 0}> --> <{0}>
+  | ST_Pred_s : forall t, 
+         <{pred (succ t)}> --> <{t}>
+
+  | ST_Succ : forall t t',
+        t --> t' ->
+         <{succ t}> --> <{succ t'}>
+  | ST_Succ_const : forall (n : nat), 
+         <{succ n}> --> tm_const (S n)
+
+  | ST_MulConst : forall (n m : nat),
+         <{ n * m }> --> tm_const (n * m)
+  | ST_Mul1 : forall t1 t1' t2,
+         t1 --> t1' ->
+         <{t1 * t2}> --> <{t1' * t2}>
+  | ST_Mul2 : forall v1 t2 t2',
+         value v1 ->
+         t2 --> t2' ->
+         <{v1 * t2}> --> <{v1 * t2'}>
+
+  | ST_IfTrue : forall t1 t2,
+      <{if0 0 then t1 else t2}> --> t1
+  | ST_IfFalse : forall n t1 t2,
+      n <> 0 ->
+      <{if0 n then t1 else t2}> --> t2
+  | ST_If : forall t1 t1' t2 t3,
+      t1 --> t1' ->
+      <{if0 t1 then t2 else t3}> --> <{if0 t1' then t2 else t3}>
+where "t '-->' t'" := (step t t').
+Hint Constructors step : core.
+
+Definition multistep := (multi step).
+Notation "t1 '-->*' t2" := (multistep t1 t2) (at level 40).
+
+
+
+Definition context := partial_map ty.
+Reserved Notation "Gamma '|-' t '\in' T"
+            (at level 101, t custom stlc, T custom stlc at level 0).
+Inductive has_type : context -> tm -> ty -> Prop :=
+  | T_Var : forall Gamma x T1,
+      Gamma x = Some T1 ->
+      Gamma |- x \in T1
+  | T_Abs : forall Gamma x T1 T2 t1,
+      (x |-> T2 ; Gamma) |- t1 \in T1 ->
+      Gamma |- \x:T2, t1 \in (T2 -> T1)
+  | T_App : forall T1 T2 Gamma t1 t2,
+      Gamma |- t1 \in (T2 -> T1) ->
+      Gamma |- t2 \in T2 ->
+      Gamma |- t1 t2 \in T1
+  | T_Const : forall Gamma (n: nat),
+       Gamma |- n \in Nat
+  | T_Succ : forall Gamma t,
+       Gamma |- t \in Nat ->
+       Gamma |- succ t \in Nat
+  | T_Pred : forall Gamma t,
+       Gamma |- t \in Nat ->
+       Gamma |- pred t \in Nat
+  | T_Mult : forall t1 t2 Gamma,
+       Gamma |- t1 \in Nat ->
+       Gamma |- t2 \in Nat ->
+       Gamma |- t1 * t2 \in Nat
+  | T_If : forall t1 t2 t3 T1 Gamma,
+       Gamma |- t1 \in Nat ->
+       Gamma |- t2 \in T1 ->
+       Gamma |- t3 \in T1 ->
+       Gamma |- if0 t1 then t2 else t3 \in T1
+where "Gamma '|-' t '\in' T" := (has_type Gamma t T).
+Hint Constructors has_type : core.
+
+
+Inductive appears_free_in (x : string) : tm -> Prop :=
+  | afi_var : appears_free_in x <{x}>
+  | afi_app1 : forall t1 t2,
+      appears_free_in x t1 ->
+      appears_free_in x <{t1 t2}>
+  | afi_app2 : forall t1 t2,
+      appears_free_in x t2 ->
+      appears_free_in x <{t1 t2}>
+  | afi_abs : forall y T1 t1,
+      y <> x ->
+      appears_free_in x t1 ->
+      appears_free_in x <{\y:T1, t1}>
+  | afi_if1 : forall t1 t2 t3,
+      appears_free_in x t1 ->
+      appears_free_in x <{if0 t1 then t2 else t3}>
+  | afi_if2 : forall t1 t2 t3,
+      appears_free_in x t2 ->
+      appears_free_in x <{if0 t1 then t2 else t3}>
+  | afi_if3 : forall t1 t2 t3,
+      appears_free_in x t3 ->
+      appears_free_in x <{if0 t1 then t2 else t3}>
+  | afi_succ : forall t,
+      appears_free_in x t ->
+      appears_free_in x <{succ t}>
+  | afi_pred : forall t,
+      appears_free_in x t ->
+      appears_free_in x <{pred t}>
+  | afi_mult1 : forall t1 t2,
+      appears_free_in x t1 ->
+      appears_free_in x <{t1 * t2}>
+  | afi_mult2 : forall t1 t2,
+      appears_free_in x t2 ->
+      appears_free_in x <{t1 * t2}>.
+Hint Constructors appears_free_in : core.
+
+Definition closed (t:tm) :=   forall x, ~(appears_free_in x t).
+
+Lemma weakening : forall Gamma Gamma' t T,
+     inclusion Gamma Gamma' ->
+     Gamma |- t \in T ->
+     Gamma' |- t \in T.
+Proof.
+  intros Gamma Gamma' t T H Ht.
+  generalize dependent Gamma'.
+  induction Ht; eauto using inclusion_update.
+Qed.
+
+Lemma weakening_empty : forall Gamma t T,
+     empty |- t \in T ->
+     Gamma |- t \in T.
+Proof.
+  intros Gamma t T.
+  eapply weakening.
+  discriminate.
+Qed.
+
+Lemma substitution_preserves_typing : forall Gamma x U t v T,
+  (x |-> U ; Gamma) |-  t \in T ->
+  empty |- v \in U ->
+  Gamma |- [x:=v]t \in T.
+Proof.
+  intros G x U t.
+  generalize dependent G.
+  generalize dependent x.
+  generalize dependent U.
+  induction t; intros U x G v T Ht Hv; simpl.
+  - (*| tm_var *)
+    destruct (eqb_stringP x s); subst.
+    + inversion Ht; subst.
+      rewrite update_eq in H1.
+      injection H1 as H1; subst.
+      apply weakening_empty.
+      assumption.
+    + inversion Ht; subst.
+      rewrite update_neq in H1; try (apply n).
+      constructor.
+      assumption.
+  - (*| tm_app *)
+    inversion Ht; subst.
+    eapply T_App.
+    + apply IHt1 with U; try (apply Hv).
+      apply H2.
+    + apply IHt2 with U; try (apply Hv).
+      apply H4.
+  - (*| tm_abs *)
+    inversion Ht; subst.
+    destruct (eqb_stringP x s); subst.
+    + apply T_Abs.
+      rewrite update_shadow in H4.
+      assumption.
+    + apply T_Abs.
+      apply IHt with U; try (apply Hv).
+      rewrite update_permute.
+        assumption.
+        intro Hc. symmetry in Hc. apply n. apply Hc.
+  - (*| tm_const *)
+    inversion Ht; subst.
+    constructor.
+  - (*| tm_succ *)
+    inversion Ht; subst.
+    constructor.
+    apply IHt with U; try (apply Hv).
+    assumption.
+  - (*| tm_pred *)
+    inversion Ht; subst.
+    constructor.
+    apply IHt with U; try (apply Hv).
+    assumption.
+  - (*| tm_mult *)
+    inversion Ht; subst.
+    eapply T_Mult.
+    + apply IHt1 with U; try (apply Hv).
+      apply H2.
+    + apply IHt2 with U; try (apply Hv).
+      apply H4.
+  - (*| tm_if0 *)
+    inversion Ht; subst.
+    eapply T_If.
+    + apply IHt1 with U; try (apply Hv).
+      apply H3.
+    + apply IHt2 with U; try (apply Hv).
+      apply H5.
+    + apply IHt3 with U; try (apply Hv).
+      apply H6.
+Qed.
+
+Theorem preservation : forall t t' T,
+  empty |- t \in T ->
+  t --> t' ->
+  empty |- t' \in T.
+Proof.
+Admitted.
+
+Theorem progress : forall t T,
+  empty |- t \in T ->
+  value t \/ exists t', t --> t'.
+Proof.
+Admitted.
+
+
+End STLCArith.
+
